src/Bedrock/Field/Synthesis/Examples/p256_64.v
@@ -2,26 +2,27 @@ Require Import Coq.ZArith.ZArith.
 Require Import Coq.Strings.String.
 Require Import Crypto.Bedrock.Field.Synthesis.Generic.WordByWordMontgomery.
 Require Import Crypto.Bedrock.Field.Synthesis.Specialized.WordByWordMontgomery.
+Require Import Crypto.Bedrock.Field.Translation.Parameters.Defaults64.
 Local Open Scope Z_scope.
 
+Local Existing Instances default_parameters default_parameters_ok.
 Local Definition m := 2^256 - 2^224 + 2^192 + 2^96 - 1.
-Local Definition machine_wordsize := 64.
 Local Definition prefix := "p256_"%string. (* placed before function names *)
 
 Instance names : names_of_operations.
-  make_names_of_operations prefix. Defined.
+Proof.  make_names_of_operations prefix. Defined.
 
-Definition ops : wbwmontgomery_reified_ops m machine_wordsize.
-  make_reified_ops. Time Defined.
+Definition ops : wbwmontgomery_reified_ops m.
+Proof.  make_reified_ops. Time Defined.
 
 Instance p256_bedrock2_funcs : bedrock2_wbwmontgomery_funcs.
-funcs_from_ops ops. Defined.
+Proof. funcs_from_ops ops. Defined.
 
 Instance p256_bedrock2_specs : bedrock2_wbwmontgomery_specs.
-specs_from_ops ops m. Defined.
+Proof. specs_from_ops ops m. Defined.
 
 Instance p256_bedrock2_correctness : bedrock2_wbwmontgomery_correctness.
-prove_correctness ops m machine_wordsize. Defined.
+Proof. prove_correctness ops m. Qed.
 
 (*
 Require Import bedrock2.NotationsCustomEntry.
