src/Bedrock/Field/Common/Names/MakeNames.v
@@ -18,7 +18,9 @@ Import ListNotations.
 Existing Instances rep.Z rep.listZ_mem.
 
 Section with_parameters.
-  Context {p : Types.parameters}.
+  Context 
+    {width BW word mem locals env ext_spec varname_gen error}
+   `{parameters_sentinel : @parameters width BW word mem locals env ext_spec varname_gen error}.
   Context {inname_gen outname_gen : nat -> string}.
 
   Fixpoint make_names
@@ -76,8 +78,7 @@ Section with_parameters.
         repeat match goal with
                | _ => progress cbn [fst snd]
                | |- ~ PropSet.singleton_set _ _ =>
-                 apply disjoint_singleton_r_iff;
-                   solve [auto using disjoint_singleton_singleton]
+                 apply disjoint_singleton_r_iff, disjoint_singleton_singleton; auto
                | |- ~ PropSet.union _ _ _ =>
                  apply not_union_iff; split; solve [auto]
                | _ => progress break_innermost_match
