src/Bedrock/Field/Translation/Cmd.v
@@ -15,7 +15,9 @@ Import API.Compilers.
 Import Types.Notations.
 
 Section Cmd.
-  Context {p : Types.parameters}.
+  Context 
+    {width BW word mem locals env ext_spec varname_gen error}
+   `{parameters_sentinel : @parameters width BW word mem locals env ext_spec varname_gen error}.
   Existing Instance Types.rep.Z.
   Existing Instance Types.rep.listZ_local. (* local list representation *)
 
